Expose data invariants via imreference
This patch also updates the interface in FStar.Monotonic.HyperStack to operate over
imreferences and exposes a compatibility layer for existing code.

ulib/FStar.Monotonic.HyperStack.fst
@@ -3,6 +3,7 @@ module FStar.Monotonic.HyperStack
 open FStar.Preorder
 open FStar.DataInvariant
 open FStar.Monotonic.HyperHeap
+
 module M  = FStar.Map
 module HH = FStar.Monotonic.HyperHeap
 
@@ -20,14 +21,14 @@ let is_below r1 r2      = r2 `is_above` r1
 let is_strictly_below r1 r2 = r1 `is_below` r2 && r1<>r2
 let is_strictly_above r1 r2 = r1 `is_above` r2 && r1<>r2
 
-let downward_closed (h:HH.t) = 
+let downward_closed (h:HH.t) =
   forall (r:rid). r `is_in` h  //for any region in the memory
         ==> (r=HH.root    //either is the root
-	    \/ (forall (s:rid). r `is_above` s  //or, any region beneath it
-			  /\ s `is_in` h   //that is also in the memory
-		     ==> (is_stack_region r = is_stack_region s))) //must be of the same flavor as itself
+      \/ (forall (s:rid). r `is_above` s  //or, any region beneath it
+        /\ s `is_in` h   //that is also in the memory
+         ==> (is_stack_region r = is_stack_region s))) //must be of the same flavor as itself
 
-let is_tip (tip:HH.rid) (h:HH.t) = 
+let is_tip (tip:HH.rid) (h:HH.t) =
   (is_stack_region tip \/ tip=HH.root)                                  //the tip is a stack region, or the root
   /\ tip `is_in` h                                                      //the tip is active
   /\ (forall (r:sid). r `is_in` h <==> r `is_above` tip)                      //any other sid activation is a above (or equal to) the tip
@@ -39,24 +40,24 @@ noeq type mem =
        -> tip:rid{tip `is_tip` h}                                                   //the id of the current top-most region
        -> mem
 
-let empty_mem (m:HH.t) = 
-  let empty_map = Map.restrict (Set.empty) m in 
-  let h = Map.upd empty_map HH.root Heap.emp in 
-  let tip = HH.root in 
+let empty_mem (m:HH.t) =
+  let empty_map = Map.restrict (Set.empty) m in
+  let h = Map.upd empty_map HH.root Heap.emp in
+  let tip = HH.root in
   HS h tip
- 
-let test0 (m:mem) (r:rid{r `is_above` m.tip}) = 
+
+let test0 (m:mem) (r:rid{r `is_above` m.tip}) =
     assert (r `is_in` m.h)
 
-let test1 (m:mem) (r:rid{r `is_above` m.tip}) = 
+let test1 (m:mem) (r:rid{r `is_above` m.tip}) =
     assert (r=HH.root \/ is_stack_region r)
 
-let test2 (m:mem) (r:sid{m.tip `is_above` r /\ m.tip <> r}) =  
+let test2 (m:mem) (r:sid{m.tip `is_above` r /\ m.tip <> r}) =
    assert (~ (r `is_in` m.h))
 
 let dc_elim (h:HH.t{downward_closed h}) (r:rid{r `is_in` h /\ r <> HH.root}) (s:rid)
   : Lemma (r `is_above` s /\ s `is_in` h ==> is_stack_region r = is_stack_region s)
-  = ()	  
+  = ()
 
 let test3 (m:mem) (r:rid{r <> HH.root /\ is_eternal_region r /\ m.tip `is_above` r /\ is_stack_region m.tip})
   : Lemma (~ (r `is_in` m.h))
@@ -68,7 +69,7 @@ let test4 (m:mem) (r:rid{r <> HH.root /\ is_eternal_region r /\ r `is_above` m.t
 
 let eternal_region_does_not_overlap_with_tip (m:mem) (r:rid{is_eternal_region r /\ not (HH.disjoint r m.tip) /\ r<>HH.root /\ is_stack_region m.tip})
   : Lemma (requires True)
-	  (ensures (~ (r `is_in` m.h)))
+    (ensures (~ (r `is_in` m.h)))
   = root_has_color_zero()
 
 let poppable m = m.tip <> HH.root
@@ -89,22 +90,35 @@ let pop (m0:mem{poppable m0}) : GTot mem =
   let tip0 = m0.tip in
   let tip1 = HH.parent tip0 in
   assert (forall (r:sid). Map.contains h1 r ==>
-  	    (forall (s:sid). includes s r ==> Map.contains h1 s));
+        (forall (s:sid). includes s r ==> Map.contains h1 s));
   HS h1 tip1
 
-//A (reference a) may reside in the stack or heap, and may be manually managed
-noeq type mreference (a:Type) (rel:preorder a) =
-  // TODO: generalize mreference to support data invariant
-  | MkRef : id:rid -> ref:HH.mrref id a (FStar.Heap.trivial_invariant a) rel -> mreference a rel
+// A (reference a) may reside in the stack or heap, and may be manually managed.
+//
+// This is the fully general reference type which supports both a monotonic relation
+// and an data invariant.
+//
+// i(nvariant)m(onotonic)reference
+noeq type imreference (a:Type) (inv:data_inv a) (rel:preorder a) =
+| MkRef : id:rid -> ref:HH.mrref id a inv rel -> imreference a inv rel
 
-let is_mm (#a:Type) (#rel:preorder a) (r:mreference a rel) :GTot bool = HH.is_mm r.ref
+// A compatibility layer, a mreference is just an imreference where the data invariant is trivial.
+let mreference (a:Type) (rel:preorder a) = imreference a (FStar.Heap.trivial_invariant a) rel
+
+let is_mm (#a:Type) (#inv:data_inv a) (#rel:preorder a) (r:imreference a inv rel) :GTot bool = HH.is_mm r.ref
 
 //adding (not s.mm) to stackref and ref so as to keep their semantics as is
-let mstackref (a:Type) (rel:preorder a) = s:mreference a rel{ is_stack_region s.id && not (is_mm s) }
-let mref (a:Type) (rel:preorder a) = s:mreference a rel{is_eternal_region s.id && not (is_mm s)}
+let imstackref (a:Type) (inv:data_inv a) (rel:preorder a) = s:imreference a inv rel{ is_stack_region s.id && not (is_mm s) }
+let mstackref (a:Type) (rel:preorder a) = imstackref a (FStar.Heap.trivial_invariant a) rel
 
-let mmmstackref (a:Type) (rel:preorder a) = s:mreference a rel{is_stack_region s.id && is_mm s }
-let mmmref (a:Type) (rel:preorder a) = s:mreference a rel{is_eternal_region s.id && is_mm s}
+let imref (a:Type) (inv:data_inv a) (rel:preorder a) = s:imreference a inv rel{is_eternal_region s.id && not (is_mm s)}
+let mref (a:Type) (rel:preorder a) = imref a (FStar.Heap.trivial_invariant a) rel
+
+let immmstackref (a:Type) (inv:data_inv a) (rel:preorder a) = s:imreference a inv rel{is_stack_region s.id && is_mm s }
+let mmmstackref (a:Type) (rel:preorder a) = immmstackref a (FStar.Heap.trivial_invariant a) rel
+
+let immmref (a:Type) (inv:data_inv a) (rel:preorder a) = s:imreference a inv rel{is_eternal_region s.id && is_mm s}
+let mmmref (a:Type) (rel:preorder a) = immmref a (FStar.Heap.trivial_invariant a) rel
 
 (*
  * The Map.contains conjunct is necessary to prove that upd
@@ -123,11 +137,11 @@ let live_region (m:mem) (i:rid) =
 let weak_live_region (m:mem) (i:rid) =
   is_eternal_region i \/ i `is_above` m.tip
 
-let contains (#a:Type) (#rel:preorder a) (m:mem) (s:mreference a rel) =
+let contains (#a:Type) (#inv:data_inv a) (#rel:preorder a) (m:mem) (s:imreference a inv rel) =
   live_region m s.id
   /\ HH.contains_ref s.ref m.h
 
-let unused_in (#a:Type) (#rel:preorder a) (r:mreference a rel) (h:mem) =
+let unused_in (#a:Type) (#inv:data_inv a) (#rel:preorder a) (r:imreference a inv rel) (h:mem) =
   ~ (live_region h r.id) \/
   HH.unused_in r.ref h.h
 
@@ -142,18 +156,18 @@ let weak_live_region_implies_eternal_or_in_map r m = ()
  * If the reference is manually managed, we must prove Heap.contains
  * before reading the ref.
  *)
-let weak_contains (#a:Type) (#rel:preorder a) (m:mem) (s:mreference a rel) =
+let weak_contains (#a:Type) (#inv:data_inv a) (#rel:preorder a) (m:mem) (s:imreference a inv rel) =
   weak_live_region m s.id /\
   (if is_mm s then HH.weak_contains_ref s.ref m.h else True)
 
 (*
  * AR: why is this not enforcing live_region ?
  *)
-let sel (#a:Type) (#rel:preorder a) (m:mem) (s:mreference a rel)
+let sel (#a:Type) (#inv:data_inv a) (#rel:preorder a) (m:mem) (s:imreference a inv rel)
   : GTot a
   = m.h.[s.ref]
 
-let upd (#a:Type) (#rel:preorder a) (m:mem) (s:mreference a rel{live_region m s.id}) (v:a{rel (sel m s) v})
+let upd (#a:Type) (#inv:data_inv a) (#rel:preorder a) (m:mem) (s:imreference a inv rel{live_region m s.id}) (v:a{rel (sel m s) v})
   : GTot mem
   = HS (m.h.[s.ref] <- v) m.tip
 
@@ -174,6 +188,7 @@ let equal_stack_domains (m0:mem) (m1:mem) =
 
 let lemma_equal_stack_domains_trans (m0:mem) (m1:mem) (m2:mem) : Lemma
   (requires (equal_stack_domains m0 m1 /\ equal_stack_domains m1 m2))
+
   (ensures  (equal_stack_domains m0 m2))
   [SMTPat (equal_stack_domains m0 m1); SMTPat (equal_stack_domains m1 m2)]
   = ()
@@ -190,7 +205,7 @@ let heap_only (m0:mem) =
   m0.tip = HH.root
 
 let top_frame (m:mem) = Map.sel m.h m.tip
-  
+
 let fresh_frame (m0:mem) (m1:mem) =
   not (Map.contains m0.h m1.tip)
   /\ HH.parent m1.tip = m0.tip
@@ -198,8 +213,8 @@ let fresh_frame (m0:mem) (m1:mem) =
 
 let modifies_drop_tip (m0:mem) (m1:mem) (m2:mem) (s:Set.set rid)
     : Lemma (fresh_frame m0 m1 /\
-	     modifies_transitively (Set.union s (Set.singleton m1.tip)) m1 m2 ==> 
-	     modifies_transitively s m0 (pop m2))
+       modifies_transitively (Set.union s (Set.singleton m1.tip)) m1 m2 ==>
+       modifies_transitively s m0 (pop m2))
     = ()
 
 let lemma_pop_is_popped (m0:mem{poppable m0})
@@ -207,40 +222,40 @@ let lemma_pop_is_popped (m0:mem{poppable m0})
   = let m1 = pop m0 in
     assert (Set.equal (Map.domain m1.h) (remove_elt (Map.domain m0.h) m0.tip))
 
-type s_mref (i:rid) (a:Type) (rel:preorder a) = s:mreference a rel{s.id = i}
+type s_mref (i:rid) (a:Type) (inv:data_inv a) (rel:preorder a) = s:imreference a inv rel{s.id = i}
 
-let frameOf #a #rel (s:mreference a rel) = s.id
+let frameOf #a #inv #rel (s:imreference a inv rel) = s.id
 
-let as_ref #a #rel (x:mreference a rel)  : GTot (Heap.mref a (FStar.Heap.trivial_invariant a) rel) = HH.as_ref #a #x.id x.ref
-let as_addr #a #rel (x:mreference a rel) : GTot nat = Heap.addr_of (HH.as_ref #a #x.id x.ref)
+let as_ref #a #inv #rel (x:imreference a inv rel)  : GTot (Heap.mref a inv rel) = HH.as_ref #a #x.id x.ref
+let as_addr #a #inv #rel (x:imreference a inv rel) : GTot nat = Heap.addr_of (HH.as_ref #a #x.id x.ref)
 let modifies_one id h0 h1 = HH.modifies_one id h0.h h1.h
 let modifies_ref (id:rid) (s:Set.set nat) (h0:mem) (h1:mem) =
   HH.modifies_rref id s h0.h h1.h /\ h1.tip=h0.tip
 
-let lemma_upd_1 #a #rel (h:mem) (x:mreference a rel) (v:a{rel (sel h x) v}) : Lemma
+let lemma_upd_1 #a #inv #rel (h:mem) (x:imreference a inv rel) (v:a{rel (sel h x) v}) : Lemma
   (requires (contains h x))
   (ensures (contains h x
-	    /\ modifies_one (frameOf x) h (upd h x v)
-	    /\ modifies_ref (frameOf x) (Set.singleton (as_addr x)) h (upd h x v)
-	    /\ sel (upd h x v) x == v ))
+      /\ modifies_one (frameOf x) h (upd h x v)
+      /\ modifies_ref (frameOf x) (Set.singleton (as_addr x)) h (upd h x v)
+      /\ sel (upd h x v) x == v ))
   [SMTPat (upd h x v); SMTPatT (contains h x)]
   = ()
 
-let lemma_upd_2 (#a:Type) (#rel:preorder a) (h:mem) (x:mreference a rel) (v:a{rel (sel h x) v}) : Lemma
+let lemma_upd_2 (#a:Type) (#inv:data_inv a) (#rel:preorder a) (h:mem) (x:imreference a inv rel) (v:a{rel (sel h x) v}) : Lemma
   (requires (frameOf x = h.tip /\ x `unused_in` h))
   (ensures (frameOf x = h.tip
-	    /\ modifies_one h.tip h (upd h x v)
-	    /\ modifies_ref h.tip Set.empty h (upd h x v)
-	    /\ sel (upd h x v) x == v ))
+      /\ modifies_one h.tip h (upd h x v)
+      /\ modifies_ref h.tip Set.empty h (upd h x v)
+      /\ sel (upd h x v) x == v ))
   [SMTPat (upd h x v); SMTPatT (x `unused_in` h)]
   = ()
 
-val lemma_live_1: #a:Type ->  #a':Type -> #rel:preorder a -> #rel':preorder a'
-                  -> h:mem -> x:mreference a rel -> x':mreference a' rel' -> Lemma
+val lemma_live_1: #a:Type ->  #a':Type -> #inv:data_inv a -> #inv':data_inv a' -> #rel:preorder a -> #rel':preorder a'
+                  -> h:mem -> x:imreference a inv rel -> x':imreference a' inv' rel' -> Lemma
   (requires (contains h x /\ x' `unused_in` h))
   (ensures  (x.id <> x'.id \/ ~ (as_ref x === as_ref x')))
   [SMTPat (contains h x); SMTPat (x' `unused_in` h)]
-let lemma_live_1 #a #a' #rel #rel' h x x' = ()
+let lemma_live_1 #a #a' #rel #rel' #inv #inv' h x x' = ()
 
 let above_tip_is_live (#a:Type) (#rel:preorder a) (m:mem) (x:mreference a rel) : Lemma
   (requires (x.id `is_above` m.tip))
@@ -250,18 +265,18 @@ let above_tip_is_live (#a:Type) (#rel:preorder a) (m:mem) (x:mreference a rel) :
 (*
  * AR: relating contains and weak_contains.
  *)
-let contains_implies_weak_contains (#a:Type) (#rel:preorder a) (h:mem) (x:mreference a rel) :Lemma
+let contains_implies_weak_contains (#a:Type) (#inv:data_inv a) l(#rel:preorder a) (h:mem) (x:imreference a inv rel) :Lemma
   (requires (True))
   (ensures (contains h x ==> weak_contains h x))
   [SMTPatOr [[SMTPat (contains h x)]; [SMTPat (weak_contains h x)]] ]
   = ()
 
 noeq type some_ref =
-| Ref : #a:Type0 -> #rel:preorder a -> mreference a rel -> some_ref
+| Ref : #a:Type0 -> #inv:data_inv a -> #rel:preorder a -> imreference a inv rel -> some_ref
 
 let some_refs = list some_ref
 
-let rec regions_of_some_refs (rs:some_refs) : Tot (Set.set rid) = 
+let rec regions_of_some_refs (rs:some_refs) : Tot (Set.set rid) =
   match rs with
   | [] -> Set.empty
   | (Ref r)::tl -> Set.union (Set.singleton r.id) (regions_of_some_refs tl)
@@ -279,20 +294,20 @@ unfold let mods (rs:some_refs) h0 h1 =
 
 ////////////////////////////////////////////////////////////////////////////////
 let eternal_disjoint_from_tip (h:mem{is_stack_region h.tip})
-			      (r:rid{is_eternal_region r /\
-				     r<>HH.root /\
-				     r `is_in` h.h})
+            (r:rid{is_eternal_region r /\
+             r<>HH.root /\
+             r `is_in` h.h})
    : Lemma (HH.disjoint h.tip r)
    = ()
-   
+
 ////////////////////////////////////////////////////////////////////////////////
 #set-options "--initial_fuel 0 --max_fuel 0 --log_queries"
-let f (a:Type0) (b:Type0) (rel_a:preorder a) (rel_b:preorder b) (rel_n:preorder nat)
-                          (x:mreference a rel_a) (x':mreference a rel_a) 
-			  (y:mreference b rel_b) (z:mreference nat rel_n) 
-			  (h0:mem) (h1:mem) = 
+let f (a:Type0) (b:Type0) (inv_a inv_a' :data_inv a) (inv_b : data_inv b) (inv_n : data_inv nat) (rel_a:preorder a) (rel_b:preorder b) (rel_n:preorder nat)
+                          (x:imreference a inv_a rel_a) (x':imreference a inv_a' rel_a)
+        (y:imreference b inv_b rel_b) (z:imreference nat inv_n rel_n)
+        (h0:mem) (h1:mem) =
   assume (h0 `contains` x);
-  assume (h0 `contains` x');  
+  assume (h0 `contains` x');
   assume (as_addr x <> as_addr x');
   assume (x.id == x'.id);
   assume (x.id <> y.id);
@@ -305,8 +320,8 @@ let f (a:Type0) (b:Type0) (rel_a:preorder a) (rel_b:preorder b) (rel_n:preorder 
   //see for example the assertion above that doesn't succeed
   assume (modifies_ref x.id (Set.singleton (as_addr x)) h0 h1);
   assert (modifies (Set.union (Set.singleton x.id)
-  			      (Set.union (Set.singleton y.id)
-  					 (Set.singleton z.id))) h0 h1);
+              (Set.union (Set.singleton y.id)
+             (Set.singleton z.id))) h0 h1);
   ()
 
 
@@ -314,7 +329,7 @@ let f (a:Type0) (b:Type0) (rel_a:preorder a) (rel_b:preorder b) (rel_n:preorder 
   //assert (sel h0 x' == sel h1 x')
 
 (* let f2 (a:Type0) (b:Type0) (x:reference a) (y:reference b) *)
-(* 			   (h0:mem) (h1:mem) =  *)
+(*         (h0:mem) (h1:mem) =  *)
 (*   assume (HH.disjoint (frameOf x) (frameOf y)); *)
 (*   assume (mods [Ref x; Ref y] h0 h1); *)
 (*  //-------------------------------------------------------------------------------- *)
@@ -335,7 +350,7 @@ let f (a:Type0) (b:Type0) (rel_a:preorder a) (rel_b:preorder b) (rel_n:preorder 
 (* #reset-options "--log_queries --initial_fuel 0 --max_fuel 0 --initial_ifuel 0 --max_ifuel 0" *)
 (* #set-options "--debug FStar.HyperStack --debug_level print_normalized_terms" *)
 (* let f3 (a:Type0) (b:Type0) (x:reference a) *)
-(* 			   (h0:mem) (h1:mem) =  *)
+(*         (h0:mem) (h1:mem) =  *)
 (*   assume (mods_2 [Ref x] h0 h1); *)
 (*  //-------------------------------------------------------------------------------- *)
 (*   assert (modifies_ref x.id (TSet.singleton (as_aref x)) h0 h1) *)
